examples/low-level/Chacha.fst
@@ -17,6 +17,8 @@ let u8 = UInt8.t
 let uint32s = buffer u32
 let bytes = buffer u8
 
+//#set-options "--lax" // OK
+
 (** Infix operators and helping lemmas **)
 // Needs to be instanciated differently
 assume MaxUint32: FStar.UInt.max_int 32 = 4294967295
@@ -117,56 +119,113 @@ let op_Hat_Star (a: u32) (b: u32): Pure u32
   op_Star_Hat a b
 
 #reset-options "--z3timeout 20"
+//#set-options "--lax" // OK
 
-val bytes_of_uint32s: output:bytes -> m:uint32s{disjoint output m} -> len:u32{op_Multiply 4 (v len)<=length output /\ v len<=length m} -> STL unit
+val bytes_of_uint32s: output:bytes -> m:uint32s{disjoint output m} -> len:u32{v len <=length output /\ v len<=op_Multiply 4 (length m)} -> STL unit
   (requires (fun h -> live h output /\ live h m))
   (ensures (fun h0 _ h1 -> live h0 output /\ live h0 m /\ live h1 output /\ live h1 m
     /\ modifies_1 output h0 h1 ))
-let rec bytes_of_uint32s output m len =
-  if len =^ 0ul then ()
-  else 
-    begin
-      let l = len -^ 1ul in
-      let x = index m l in
+let rec bytes_of_uint32s output m l =
+  if UInt32.gte l 4ul then begin
+    let l = UInt32.sub l 4ul in
+    let x = index m (UInt32.div l 4ul) in
+    let b0 = uint32_to_uint8 (x &^ 255ul) in
+    let b1 = uint32_to_uint8 ((x ^>> 8ul) &^ 255ul) in
+    let b2 = uint32_to_uint8 ((x ^>> 16ul) &^ 255ul) in
+    let b3 = uint32_to_uint8 ((x ^>> 24ul) &^ 255ul) in
+    upd output l b0;
+    upd output (l +^ 1ul) b1;
+    upd output (l +^ 2ul) b2;
+    upd output (l +^ 3ul) b3;
+    bytes_of_uint32s output m l 
+  end
+  else begin
+    if UInt32.eq l 0ul then ()
+    else begin
+      let x = index m (UInt32.div l 4ul) in
       let b0 = uint32_to_uint8 (x &^ 255ul) in
-      let b1 = uint32_to_uint8 ((x ^>> 8ul) &^ 255ul) in
-      let b2 = uint32_to_uint8 ((x ^>> 16ul) &^ 255ul) in
-      let b3 = uint32_to_uint8 ((x ^>> 24ul) &^ 255ul) in
-      let l4 = l ^* 4ul in
-      upd output l4 b0; 
-      upd output (l4 +^ 1ul) b1;
-      upd output (l4 +^ 2ul) b2;
-      upd output (l4 +^ 3ul) b3;
-      bytes_of_uint32s output m l
+      upd output 0ul b0;
+      if UInt32.gte l 2ul then begin
+	let b1 = uint32_to_uint8 ((x ^>> 8ul) &^ 255ul) in
+	upd output (1ul) b1;
+	if UInt32.gte l 3ul then begin
+	  let b2 = uint32_to_uint8 ((x ^>> 16ul) &^ 255ul) in
+	  upd output (2ul) b2
+	end
+        else ()
+      end
+      else ()
     end
+  end
+
+(* val bytes_of_uint32s: output:bytes -> m:uint32s{disjoint output m} -> len:u32{op_Multiply 4 (v len)<=length output /\ v len<=length m} -> STL unit *)
+(*   (requires (fun h -> live h output /\ live h m)) *)
+(*   (ensures (fun h0 _ h1 -> live h0 output /\ live h0 m /\ live h1 output /\ live h1 m *)
+(*     /\ modifies_1 output h0 h1 )) *)
+(* let rec bytes_of_uint32s output m len = *)
+(*   if len =^ 0ul then () *)
+(*   else  *)
+(*     begin *)
+(*       let l = len -^ 1ul in *)
+(*       let x = index m l in *)
+(*       let b0 = uint32_to_uint8 (x &^ 255ul) in *)
+(*       let b1 = uint32_to_uint8 ((x ^>> 8ul) &^ 255ul) in *)
+(*       let b2 = uint32_to_uint8 ((x ^>> 16ul) &^ 255ul) in *)
+(*       let b3 = uint32_to_uint8 ((x ^>> 24ul) &^ 255ul) in *)
+(*       let l4 = l ^* 4ul in *)
+(*       upd output l4 b0;  *)
+(*       upd output (l4 +^ 1ul) b1; *)
+(*       upd output (l4 +^ 2ul) b2; *)
+(*       upd output (l4 +^ 3ul) b3; *)
+(*       bytes_of_uint32s output m l *)
+(*     end *)
 
 #reset-options
+//#set-options "--lax" // OK
 
 val xor_bytes: output:bytes -> in1:bytes -> in2:bytes{disjoint in1 in2 /\ disjoint in1 output /\ disjoint in2 output} -> len:u32{v len <= length output /\ v len <= length in1 /\ v len <= length in2} -> STL unit
   (requires (fun h -> live h output /\ live h in1 /\ live h in2))
-  (ensures  (fun h0 _ h1 -> live h0 output /\ live h0 in1 /\ live h0 in2 
+  (ensures  (fun h0 _ h1 -> live h0 output /\ live h0 in1 /\ live h0 in2
     /\ live h1 output /\ live h1 in1 /\ live h1 in2
-    /\ modifies_1 output h0 h1
-    (* /\ (forall (i:nat). i < v len ==> get h1 output i = (UInt8.logxor (get h0 in1 i) (get h0 in2 i))) *)
-   ))
+    /\ modifies_1 output h0 h1 ))
 let rec xor_bytes output in1 in2 len =
   let h0 = HST.get() in
   if len =^ 0ul then ()
   else
     begin
-      let i = len -^ 1ul in 
+      let i = len -^ 1ul in
       let in1i = index in1 i in
       let in2i = index in2 i in
       let oi = UInt8.logxor in1i in2i in
-      upd output i oi; 
+      upd output i oi;
       let h1 = HST.get() in
       no_upd_lemma_1 h0 h1 output in1;
       no_upd_lemma_1 h0 h1 output in2;
       xor_bytes output in1 in2 i
     end
 
-// TODO 
-(* #set-options "--lax" *)
+val xor_bytes_2: output:bytes -> in1:bytes{disjoint in1 output} -> 
+  len:u32{v len <= length output /\ v len <= length in1} -> STL unit
+  (requires (fun h -> live h output /\ live h in1))
+  (ensures  (fun h0 _ h1 -> live h0 output /\ live h0 in1 /\ live h1 output /\ live h1 in1
+    /\ modifies_1 output h0 h1 ))
+let rec xor_bytes_2 output in1 len =
+  let h0 = HST.get() in
+  if len =^ 0ul then ()
+  else
+    begin
+      let i    = len -^ 1ul in
+      let in1i = index in1 i in
+      let oi   = index output i in
+      let oi   = UInt8.logxor in1i oi in
+      upd output i oi;
+      let h1 = HST.get() in
+      no_upd_lemma_1 h0 h1 output in1;
+      xor_bytes_2 output in1 i
+    end
+
+#reset-options "--z3timeout 50"
+//#set-options "--lax" // OK
 
 val initialize_state: state:uint32s{length state = 16} -> 
   key:bytes{length key = 32 /\ disjoint state key} -> counter:u32 -> 
@@ -174,11 +233,6 @@ val initialize_state: state:uint32s{length state = 16} ->
   (requires (fun h -> live h state /\ live h key /\ live h nonce))
   (ensures (fun h0 _ h1 -> live h1 state /\ modifies_1 state h0 h1))
 let initialize_state state key counter nonce =
-  (* Constant part *)
-  upd state 0ul 0x61707865ul;
-  upd state 1ul 0x3320646eul;
-  upd state 2ul 0x79622d32ul;
-  upd state 3ul 0x6b206574ul;
   (* Key part *)
   let k0 = sub key 0ul  4ul in 
   let k1 = sub key 4ul  4ul in 
@@ -188,37 +242,51 @@ let initialize_state state key counter nonce =
   let k5 = sub key 20ul 4ul in 
   let k6 = sub key 24ul 4ul in 
   let k7 = sub key 28ul 4ul in
-  (* let k0 = sub key 0ul 4ul  in  *)
-  (* let k1 = sub key 4ul 4ul  in *)
-  (* let k2 = sub key 8ul 4ul  in *)
-  (* let k3 = sub key 12ul 4ul in  *)
-  (* let k4 = sub key 16ul 4ul in  *)
-  (* let k5 = sub key 20ul 4ul in *)
-  (* let k6 = sub key 24ul 4ul in *)
-  (* let k7 = sub key 28ul 4ul in  *)
+  let k0 =  (uint32_of_bytes k0) in
+  let k1 =  (uint32_of_bytes k1) in 
+  let k2 =  (uint32_of_bytes k2) in 
+  let k3 =  (uint32_of_bytes k3) in 
+  let k4 =  (uint32_of_bytes k4) in
+  let k5 =  (uint32_of_bytes k5) in
+  let k6 =  (uint32_of_bytes k6) in
+  let k7 =  (uint32_of_bytes k7) in
   (* Nonce part *)
   let n0 = sub nonce 0ul 4ul in 
   let n1 = sub nonce 4ul 4ul in 
   let n2 = sub nonce 8ul 4ul in
+  let n0 =  (uint32_of_bytes n0) in
+  let n1 =  (uint32_of_bytes n1) in
+  let n2 =  (uint32_of_bytes n2) in
+  let h0 = HST.get() in
+  (* Constant part *)
+  upd state 0ul 0x61707865ul;
+  upd state 1ul 0x3320646eul;
+  upd state 2ul 0x79622d32ul;
+  upd state 3ul 0x6b206574ul;
+  let h1 = HST.get() in
+  cut (live h1 state /\ modifies_1 state h0 h1);
   (* Update with key *)
-  upd state 4ul  (uint32_of_bytes k0); 
-  upd state 5ul  (uint32_of_bytes k1); 
-  upd state 6ul  (uint32_of_bytes k2); 
-  upd state 7ul  (uint32_of_bytes k3); 
-  upd state 8ul  (uint32_of_bytes k4);
-  upd state 9ul  (uint32_of_bytes k5);
-  upd state 10ul (uint32_of_bytes k6);
-  upd state 11ul (uint32_of_bytes k7);
+  upd state 4ul  (k0);
+  upd state 5ul  (k1); 
+  upd state 6ul  (k2); 
+  upd state 7ul  (k3); 
+  upd state 8ul  (k4);
+  upd state 9ul  (k5);
+  upd state 10ul (k6);
+  upd state 11ul (k7);
+  let h2 = HST.get() in
+  cut (live h2 state /\ modifies_1 state h1 h2);
   (* Block counter part *)
   upd state 12ul counter; 
   (* Update with nonces *)
-  upd state 13ul (uint32_of_bytes n0);
-  upd state 14ul (uint32_of_bytes n1);
-  upd state 15ul (uint32_of_bytes n2)
+  upd state 13ul (n0);
+  upd state 14ul (n1);
+  upd state 15ul (n2)
 
 #reset-options
+//#set-options "--lax" // OK
 
-val sum_matrixes: new_state:uint32s{length new_state = 16} -> old_state:uint32s{length old_state = 16 /\ disjoint new_state old_state} -> ST unit
+val sum_matrixes: new_state:uint32s{length new_state = 16} -> old_state:uint32s{length old_state = 16 /\ disjoint new_state old_state} -> STL unit
   (requires (fun h -> live h new_state /\ live h old_state))
   (ensures (fun h0 _ h1 -> live h1 new_state /\ modifies_1 new_state h0 h1))
 let sum_matrixes m m0 =
@@ -243,7 +311,8 @@ let sum_matrixes m m0 =
 let s #t (b:buffer t) = Set.singleton (frameOf b)
 let op_Plus_Plus = Set.union
 
-#set-options "--lax" // Try large timeout
+#reset-options "--z3timeout 200"
+//#set-options "--lax" // OK with large timeout
 
 let lemma_chacha20_block (output:bytes) (state:uint32s{frameOf output <> frameOf state}) 
   (m0:uint32s{frameOf m0 <> frameOf state /\ frameOf m0 <> frameOf output})
@@ -258,17 +327,18 @@ let lemma_chacha20_block (output:bytes) (state:uint32s{frameOf output <> frameOf
   (ensures (modifies_2 output state hinit hfin /\ live hfin output /\ live hfin state ))
   = ()
 
-(* #set-options "--lax" *)
+#reset-options "--z3timeout 50"
+//#set-options "--lax" // OK modulo assume
 
-#reset-options
-
-val chacha20_block: output:bytes{length output = 64} -> 
+val chacha20_block: output:bytes -> 
   state:uint32s{length state = 16 /\ frameOf state <> frameOf output} ->
   key:bytes{length key = 32 /\ disjoint state key /\ disjoint output key} -> counter:u32 -> 
-  nonce:bytes{length nonce = 12 /\ disjoint key nonce /\ disjoint state nonce /\ disjoint nonce output} -> STL unit
+  nonce:bytes{length nonce = 12 /\ disjoint key nonce /\ disjoint state nonce /\ disjoint nonce output} -> 
+  len:u32{v len <= 64 /\ length output >= v len} ->
+  STL unit
     (requires (fun h -> live h state /\ live h output /\ live h key /\ live h nonce))
     (ensures (fun h0 _ h1 -> live h1 output /\ live h1 state /\ modifies_2 output state h0 h1 ))
-let chacha20_block output m key counter nonce =
+let chacha20_block output m key counter nonce len =
   let h0 = HST.get() in
   push_frame ();
   (* Initialize internal state *)
@@ -307,7 +377,7 @@ let chacha20_block output m key counter nonce =
   cut(modifies_1 m h3 h5);
   no_upd_lemma_1 h3 h5 m output;
   (* Serialize the state into byte stream *)
-  bytes_of_uint32s output m 16ul;
+  bytes_of_uint32s output m len;
   let h6 = HST.get() in
   cut(modifies_1 output h5 h6);
   cut(live h6 output /\ live h6 m);
@@ -320,20 +390,19 @@ let chacha20_block output m key counter nonce =
   lemma_chacha20_block output m m0 h0 h0' h1 h2 h3 h5 h6 h7; 
   assume (equal_domains h0 h7) // TODO, need lemmas about that
 
-#reset-options
-#set-options "--lax"
+#reset-options "--z3timeout 100"
+//#set-options "--lax" // OK
 
 val chacha20_encrypt_loop: 
   state:uint32s{length state = 16} -> key:bytes{length key = 32 /\ disjoint state key} -> 
   counter:u32 -> nonce:bytes{length nonce = 12 /\ disjoint state nonce /\ disjoint key nonce} -> 
   plaintext:bytes{disjoint state plaintext /\ disjoint key plaintext /\ disjoint nonce plaintext} -> 
-  ciphertext:bytes{frameOf state <> frameOf ciphertext /\ disjoint key ciphertext /\ disjoint nonce ciphertext /\ disjoint plaintext ciphertext} -> j:u32 -> max:u32{v j <= v max /\ v counter + v max < pow2 n} -> 
+  ciphertext:bytes{frameOf state <> frameOf ciphertext /\ disjoint key ciphertext /\ disjoint nonce ciphertext /\ disjoint plaintext ciphertext} -> j:u32 -> max:u32{v j <= v max /\ v counter + v max < pow2 n} ->
   STL unit
     (requires (fun h -> live h state /\ live h key /\ live h nonce /\ live h plaintext  /\ live h ciphertext
       /\ length plaintext >= (v max-v j) * 64  /\ length ciphertext >= (v max-v j) * 64 ))
     (ensures (fun h0 _ h1 -> live h1 ciphertext /\ live h1 state /\ modifies_2 ciphertext state h0 h1 ))
 let rec chacha20_encrypt_loop state key counter nonce plaintext ciphertext j max =
-  let h0 = HST.get() in
   if j =^ max then ()
   else 
     begin
@@ -342,40 +411,47 @@ let rec chacha20_encrypt_loop state key counter nonce plaintext ciphertext j max
       let ciphertext' = sub ciphertext 64ul (64ul ^* (max -^ j -^ 1ul)) in
       let plain_block = sub plaintext 0ul 64ul in
       let plaintext' = sub plaintext 64ul (64ul ^* (max -^ j -^ 1ul)) in
-      chacha20_block cipher_block state key (counter +^ j) nonce; 
+      let h0 = HST.get() in
+      cut (live h0 plaintext' /\ live h0 ciphertext');
+      cut (disjoint plaintext' cipher_block  /\ disjoint plaintext' state);
+      cut (disjoint ciphertext' cipher_block  /\ disjoint ciphertext' state);
+      chacha20_block cipher_block state key (counter +^ j) nonce 64ul;
 	(** Lemmas **)
 	let h1 = HST.get() in
-	(* aux_lemma plain_block cipher_block state; *)
-	(* (\* eq_lemma h0 h1 plain_block (only cipher_block ++ state);  *\) *)
+	aux_lemma plain_block cipher_block state;
+	eq_lemma_2 h0 h1 cipher_block state plain_block;
 	(** End lemmas **)
       (* XOR the key stream with the plaintext *)
-      xor_bytes cipher_block cipher_block plain_block 64ul; 
+      xor_bytes_2 cipher_block plain_block 64ul;
 	(** Lemmas **)
 	let h2 = HST.get() in
-	(* (\* eq_lemma h1 h2 plain_block (only cipher_block ++ state);  *\) *)
-	(* aux_lemma' state cipher_block;  *)
-	(* (\* eq_lemma h1 h2 state (only cipher_block);  *\) *)
-	(* aux_lemma nonce cipher_block state; *)
-	(* (\* eq_lemma h0 h2 nonce (only cipher_block ++ state);  *\) *)
-	(* aux_lemma key cipher_block state; *)
-	(* (\* eq_lemma h0 h2 key (only cipher_block ++ state);  *\) *)
-	(* aux_lemma plaintext' cipher_block state; *)
-	(* (\* eq_lemma h0 h2 plaintext' (only cipher_block ++ state);  *\) *)
-	(* aux_lemma ciphertext' cipher_block state; *)
-	(* (\* eq_lemma h0 h2 ciphertext' (only cipher_block ++ state);  *\) *)
+	lemma_modifies_2_1 cipher_block state h0 h1 h2;
+	(* eq_lemma_2 h1 h2 cipher_block state plain_block; *)
+	aux_lemma' state cipher_block;
+	aux_lemma key cipher_block state;
+	aux_lemma nonce cipher_block state;
+	aux_lemma plaintext' cipher_block state;
+	aux_lemma ciphertext' cipher_block state;
+	eq_lemma_1 h1 h2 cipher_block plain_block;
+	eq_lemma_1 h1 h2 cipher_block state;
+	eq_lemma_2 h0 h2 cipher_block state nonce;
+	eq_lemma_2 h0 h2 cipher_block state key;
+	eq_lemma_2 h0 h2 cipher_block state plaintext';
+	eq_lemma_2 h0 h2 cipher_block state ciphertext';
 	(** End lemmas **)
       (* Apply Chacha20 to the next blocks *)
       chacha20_encrypt_loop state key counter nonce plaintext' ciphertext' (j +^ 1ul) max;
 	(** Lemmas **)
 	let h3 = HST.get() in
-	(* aux_lemma'' state cipher_block; *)
-	(* aux_lemma'' state ciphertext'; *)
-	(* aux_lemma'' state ciphertext; *)
-	(* modifies_subbuffer_lemma h0 h2 (only state) cipher_block ciphertext; *)
-	(* modifies_subbuffer_lemma h2 h3 (only state) ciphertext' ciphertext *)
-	()
+	aux_lemma'' state cipher_block;
+	aux_lemma'' state ciphertext';
+	aux_lemma'' state ciphertext;
+	modifies_subbuffer_2 h0 h2 cipher_block state ciphertext;
+	modifies_subbuffer_2 h2 h3 ciphertext' state ciphertext
 	(** End lemmas **)
     end
+
+#reset-options "--z3timeout 100"
 
 let op_Hat_Slash a b = op_Slash_Hat a b
 let op_Hat_Percent a b = op_Percent_Hat a b
@@ -387,62 +463,63 @@ val chacha20_encrypt:
     (requires (fun h -> live h ciphertext /\ live h key /\ live h nonce /\ live h plaintext))
     (ensures (fun h0 _ h1 -> live h1 ciphertext /\ modifies_1 ciphertext h0 h1))
 let chacha20_encrypt ciphertext key counter nonce plaintext len = 
+  let hinit = HST.get() in
   push_frame ();
   let h0 = HST.get() in
+  let h0' = HST.get() in
   (* Allocate the internal state *)
   let state = create 0ul 16ul  in
   (* Compute number of iterations *)
   let max = (len ^/ 64ul) in 
   let rem = len ^% 64ul in
     (** Lemmas **)
-    (* cut (length ciphertext >= v len /\ length ciphertext >= v max * 64);  *)
-    (* cut (length plaintext >= v len /\ length plaintext >= v max * 64);  *)
+    cut (length ciphertext >= v len /\ length ciphertext >= v max * 64);
+    cut (length plaintext >= v len /\ length plaintext >= v max * 64);
     let h1 = HST.get() in
+    let h1' = HST.get() in
     (** End lemmas **)    
   (* Apply Chacha20 max times **)  
-  (* assert(disjoint state plaintext); admit() *)
+  assert(disjoint state plaintext);
   chacha20_encrypt_loop state key counter nonce plaintext ciphertext 0ul max;
     (** Lemmas **)
     let h2 = HST.get() in 
+    let h2' = HST.get() in
     assert(frameOf state = h0.tip);
-    modifies_fresh h0 h2 (only ciphertext) state;
     (** End lemmas **)
-  if rem =^ 0ul then 
-    begin
-      (** Lemmas **)
-      (* modifies_fresh_lemma h0 h2 (only ciphertext) state *)
-      ()
-      (** End lemmas **)
-    end
+  if rem =^ 0ul then begin 
+    lemma_modifies_2_0 ciphertext state h0 h1 h2;
+    cut (modifies_2_1 ciphertext h0 h2)
+  end
   else 
     begin 
+      let cipher_block = sub ciphertext (UInt32.mul 64ul max) rem in 
+      let plain_block = sub plaintext (UInt32.mul 64ul max) rem in 
+      let h0 = HST.get() in
+      chacha20_block cipher_block state key (counter +^ max) nonce rem;
 	(** Lemmas **)
-	(* eq_lemma h1 h2 plaintext (only ciphertext ++ state);  *)
-	(* eq_lemma h1 h2 key (only ciphertext ++ state);  *)
-	(* eq_lemma h1 h2 nonce (only ciphertext ++ state);  *)
+	let h1 = HST.get() in
+	aux_lemma plain_block cipher_block state;
+	eq_lemma_2 h0 h1 cipher_block state plain_block;
 	(** End lemmas **)
-      (* Apply Chacha20 to last block *)
-      let cipher_block = create 0uy 64ul in
-      let cipher_block' = sub ciphertext (max ^* 64ul) (len -^ (max ^* 64ul)) in
-      let plain_block = sub plaintext (max ^* 64ul) (len -^ (max ^* 64ul)) in
-      (* let cipher_block' = offset ciphertext (max*64) in *)
-      (* let plain_block = offset plaintext (max*64) in *)
-      chacha20_block cipher_block state key (counter +^ max) nonce; 
-	(** Lemmas **)
-	let h3 = HST.get() in
-	(* cut (v rem < 64 /\ length cipher_block >= v rem /\ v len = Prims.op_Addition (v max * 64) (v rem));  *)
-	(* cut (True /\ length plain_block >= v len - (v max * 64));  *)
-	(** End lemmas **)	
       (* XOR the key stream with the plaintext *)
-      xor_bytes cipher_block' cipher_block plain_block rem;
+      xor_bytes_2 cipher_block plain_block rem;
 	(** Lemmas **)
-	let h4 = HST.get() in 
-	aux_lemma'' state cipher_block;
-	modifies_fresh h2 h3 (only state) cipher_block
-	(* modifies_subbuffer_lemma h3 h4 empty cipher_block' ciphertext;  *)
-	(* empty_lemma ciphertext; *)
-	(* modifies_fresh h0 h4 (only ciphertext) state *)
-	(** End lemmas **)	
+	let h2 = HST.get() in
+	lemma_modifies_2_1 cipher_block state h0 h1 h2;
+	aux_lemma' state cipher_block;
+	aux_lemma key cipher_block state;
+	aux_lemma nonce cipher_block state;
+	eq_lemma_1 h1 h2 cipher_block plain_block;
+	eq_lemma_1 h1 h2 cipher_block state;
+	eq_lemma_2 h0 h2 cipher_block state nonce;
+	eq_lemma_2 h0 h2 cipher_block state key;
+	modifies_subbuffer_2 h0 h2 cipher_block state ciphertext;
+	cut (modifies_2 ciphertext state h1' h2); 
+	lemma_modifies_2_0 ciphertext state h0' h1' h2
     end;
+    let h1' = HST.get() in
     pop_frame ();
-    admit()
+    let hfin = HST.get() in
+    modifies_popped_1 ciphertext hinit h0' h1' hfin;
+    assume (equal_domains hinit hfin) // TODO, need lemmas about that
+
